Comparse.Tactic.fst
@@ -1,3 +1,4 @@
 module Comparse.Tactic
 
+include Comparse.Tactic.Attributes
 include Comparse.Tactic.Generate
